@prefix : <http://gams.uni-graz.at/o:typoo.ontology#> .
@prefix owl: <http://www.w3.org/2002/07/owl#> .
@prefix rdf: <http://www.w3.org/1999/02/22-rdf-syntax-ns#> .
@prefix xml: <http://www.w3.org/XML/1998/namespace> .
@prefix xsd: <http://www.w3.org/2001/XMLSchema#> .
@prefix rdfs: <http://www.w3.org/2000/01/rdf-schema#> .
@prefix skos: <http://www.w3.org/2004/02/skos/core#> .
@prefix terms: <http://purl.org/dc/terms/> .
@prefix typoo: <http://glossa.uni-graz.at/o:typoo.ontology#> .
@base <http://gams.uni-graz.at/o:typoo.ontology> .

<http://gams.uni-graz.at/o:typoo.ontology> rdf:type owl:Ontology ;
                                            owl:versionInfo """Version
            1.0"""^^xsd:string ;
                                            terms:creator "Frederike Neuber" .

#################################################################
#    Object Properties
#################################################################

###  http://gams.uni-graz.at/o:typoo.ontology#feature
:feature rdf:type owl:ObjectProperty ;
         owl:inverseOf :featureOf ;
         rdfs:domain [ rdf:type owl:Class ;
                       owl:unionOf ( :Type
                                     :TypeFragment
                                     :Typeface
                                   )
                     ] ;
         rdfs:range :FragmentFeature ;
         owl:propertyChainAxiom ( :part
                                  :structure
                                  :feature
                                ) ;
         rdfs:comment """A Structure Feature that characterizes a Structure Element as
            well as the related Type and the Typeface it belongs to."""@en ,
                      """Ein Strukturmerkmal, das ein Strukturelement sowie die
            zugehörige Type und die dazugehörige Schriftart charakterisiert."""@de ;
         rdfs:label "Merkmal"@de ,
                    "feature"@en .


###  http://gams.uni-graz.at/o:typoo.ontology#featureOf
:featureOf rdf:type owl:ObjectProperty ;
           rdfs:domain :FragmentFeature ;
           rdfs:range [ rdf:type owl:Class ;
                        owl:unionOf ( :Type
                                      :TypeFragment
                                      :Typeface
                                    )
                      ] ;
           rdfs:comment """A Structure Element as well as the Type it belongs to and the
            related Typeface that is also characterized by this Strcture Feature."""@en ,
                        """Ein Strukturelement sowie die dazugehörige Type und die
            zugehörige Schriftart, die ebenfalls durch dieses Strukturmerkmal gekennzeichnet
            ist."""@de ;
           rdfs:label "Merkmal von"@de ,
                      "feature Of"@en .


###  http://gams.uni-graz.at/o:typoo.ontology#formFeature
:formFeature rdf:type owl:ObjectProperty ;
             owl:inverseOf :formFeatureOf ;
             rdfs:domain :Typeface ;
             rdfs:range :CategoryForm ;
             rdfs:comment """A Form Feature that according to design conventions
            characterizes Typefaces (e.g. Stroke Constrast, Terminals, etc.)."""@en ,
                          """Ein Formularmerkmal, das nach Designkonventionen Schriften
            charakterisiert (z.B. Strichkontrast, Ausläufe, etc.)."""@de ;
             rdfs:label "Form Feature"@en ,
                        "Formenmerkmal"@de .


###  http://gams.uni-graz.at/o:typoo.ontology#formFeatureOf
:formFeatureOf rdf:type owl:ObjectProperty ;
               rdfs:domain :CategoryForm ;
               rdfs:range :Typeface ;
               rdfs:comment """A Typeface that is characterized by a Form Feature of design
            conventions."""@en ,
                            """Eine Schriftart, die durch ein Formenmerkmal gekennzeichnet
            ist."""@de ;
               rdfs:label "Formenmerkmal von"@de ,
                          "form Feature Of"@en .


###  http://gams.uni-graz.at/o:typoo.ontology#manifestation
:manifestation rdf:type owl:ObjectProperty ;
               owl:inverseOf :manifestationOf ;
               rdfs:comment """A Grapheme, an Allograph, a Font Type, a Design Type or a Graph
            in which an Archigrapheme, a Grapheme, an Allograph, a Design Type or a Font Type are
            manifested."""@en ,
                            """Ein Graphem, ein Allograph, eine Type, eine Drucktype oder ein
            Protograph, in dem sich ein Archigraphem, ein Graphem, ein Allograph, eine Type, eine
            Drucktype manifestiert."""@de ;
               rdfs:label "Manifestation"@de ,
                          "manifestation"@en .


###  http://gams.uni-graz.at/o:typoo.ontology#manifestationOf
:manifestationOf rdf:type owl:ObjectProperty ;
                 rdfs:comment """An Archigrapheme, a Grapheme, an Allograph, a Design Type or a
            Font Type which are manifested by a Grapheme, an Allograph, a Design Type, a Font Type
            or a Protoraph."""@en ,
                              """Ein Archigraphem, ein Graphem, ein Allograph, eine Type oder
            eine Drucktype, die sich durch ein Graphem, ein Allograph, eine Type, eine Drucktype
            oder einen Protographen manifestieren."""@de ;
                 rdfs:label "Manifestation von"@de ,
                            "manifestation Of"@en .


###  http://gams.uni-graz.at/o:typoo.ontology#occurence
:occurence rdf:type owl:ObjectProperty ;
           owl:inverseOf :occurenceOf ;
           owl:propertyChainAxiom ( :manifestation
                                    :part
                                    :occurence
                                  ) ,
                                  ( :occurence
                                    :subdivisionOf
                                  ) ,
                                  ( :part
                                    :occurence
                                  ) ;
           rdfs:comment """A Function Area or an Item Part in which a Protograph
            occurs."""@en ,
                        """Ein Funktionsbereich oder Exemplarteil in dem ein Protograph
            auftritt."""@de ;
           rdfs:label "Vorkommen"@de ,
                      "occurence"@en .


###  http://gams.uni-graz.at/o:typoo.ontology#occurenceOf
:occurenceOf rdf:type owl:ObjectProperty ;
             rdfs:domain :CategoryContext ;
             owl:propertyChainAxiom ( :occurenceOf
                                      :partOf
                                    ) ;
             rdfs:comment """A Protograph which occurs in an Item Part and a Function
            Area."""@en ,
                          """Ein Protograph, der in einem Funktionsbereich und einem
            Exemplarteil auftritt."""@de ;
             rdfs:label "Vorkommen von"@de ,
                        "occurence Of"@en .


###  http://gams.uni-graz.at/o:typoo.ontology#part
:part rdf:type owl:ObjectProperty ;
      owl:inverseOf :partOf ;
      rdfs:domain [ rdf:type owl:Class ;
                    owl:unionOf ( :Font
                                  :Typeface
                                )
                  ] ;
      rdfs:range [ rdf:type owl:Class ;
                   owl:unionOf ( :FontType
                                 :Type
                               )
                 ] ;
      rdfs:comment """A Type which belongs to a Typeface or a Font-Type wich belongs
            to a Font."""@en ,
                   """Eine Type, die zu einer Schriftart gehört, oder eine Drucktype
            die zu einem Schriftschnitt gehört."""@de ;
      rdfs:label "Teil"@de ,
                 "part"@en .


###  http://gams.uni-graz.at/o:typoo.ontology#partOf
:partOf rdf:type owl:ObjectProperty ;
        rdfs:domain [ rdf:type owl:Class ;
                      owl:unionOf ( :FontType
                                    :Type
                                  )
                    ] ;
        rdfs:range [ rdf:type owl:Class ;
                     owl:unionOf ( :Font
                                   :Typeface
                                 )
                   ] ;
        rdfs:comment """A Typeface to which Design Type belongs or a Font to which a
            Font Type belongs."""@en ,
                     """Eine Schriftart, zu der eine Type gehört, oder ein
            Schriftschnitt, zu dem eine Druck Type gehört."""@de ;
        rdfs:label "Teil von"@de ,
                   "part Of"@en .


###  http://gams.uni-graz.at/o:typoo.ontology#relation
:relation rdf:type owl:ObjectProperty ;
          owl:inverseOf :relation ;
          rdf:type owl:SymmetricProperty ;
          rdfs:domain :CategoryScriptIndividuals ;
          rdfs:range :CategoryScriptIndividuals ;
          owl:propertyChainAxiom ( :manifestation
                                   :manifestation
                                 ) ,
                                 ( :manifestation
                                   :manifestation
                                   :manifestation
                                 ) ,
                                 ( :manifestation
                                   :manifestation
                                   :manifestation
                                   :manifestation
                                 ) ,
                                 ( :manifestation
                                   :manifestation
                                   :manifestation
                                   :manifestation
                                   :manifestation
                                 ) ,
                                 ( :manifestation
                                   :manifestation
                                   :manifestation
                                   :manifestation
                                   :manifestation
                                   :manifestation
                                 ) ,
                                 ( :manifestationOf
                                   :manifestationOf
                                 ) ,
                                 ( :manifestationOf
                                   :manifestationOf
                                   :manifestationOf
                                 ) ,
                                 ( :manifestationOf
                                   :manifestationOf
                                   :manifestationOf
                                   :manifestationOf
                                 ) ,
                                 ( :manifestationOf
                                   :manifestationOf
                                   :manifestationOf
                                   :manifestationOf
                                   :manifestationOf
                                 ) ;
          rdfs:comment """An Archigrapheme, a Grapheme, an Allograph, a Font Type or a
            Graph which is related through a chain of manifestations with an Archigrapheme, a
            Grapheme, an Allograph, a Font Type or a Graph."""@en ,
                       """Ein Archigraphem, ein Graphem, ein Allograph, eine Desing-Type,
            Drucktype oder ein Protograph, die jeweils durch eine Eigenschafts-Kette von
            Manifestationen mit einem anderen Archigraphem, einem Graphem, einem Allographen, einer
            Type, einer Drucktype oder einem Protographen in Beziehung stehen."""@de ;
          rdfs:label "Beziehung"@de ,
                     "relation"@en .


###  http://gams.uni-graz.at/o:typoo.ontology#structure
:structure rdf:type owl:ObjectProperty ;
           owl:inverseOf :structureOf ;
           rdfs:domain :Type ;
           rdfs:range :TypeFragment ;
           rdfs:comment "A Structure Element of a Design Type."@en ,
                        "Ein Strukturelement einer Type."@de ;
           rdfs:label "Struktur"@de ,
                      "structure"@en .


###  http://gams.uni-graz.at/o:typoo.ontology#structureOf
:structureOf rdf:type owl:ObjectProperty ;
             rdfs:domain :TypeFragment ;
             rdfs:range :Type ;
             rdfs:comment "A Font Type that comprises a Structure Element."@en ,
                          """Eine Drucktype die über ein Strukturelement
            verfügt."""@de ;
             rdfs:label "Struktur von"@de ,
                        "structure Of"@en .


###  http://gams.uni-graz.at/o:typoo.ontology#style
:style rdf:type owl:ObjectProperty ;
       owl:inverseOf :styleOf ;
       rdfs:domain :Font ;
       rdfs:comment """Stilelemente, die einen Schriftschnitt nach typografischen
            Konventionen charakterisieren (z.B. Name, Dickte, Größe, etc.)"""@de ,
                    """Style elements that characterize a typeface according to
            typographical conventions (e.g. name, width, size, etc.)."""@en ;
       rdfs:label "Stil"@de ,
                  "style"@en .


###  http://gams.uni-graz.at/o:typoo.ontology#styleOf
:styleOf rdf:type owl:ObjectProperty ;
         rdfs:range :Font ;
         rdfs:comment "A Font that is chracterized by a Font Style"@en ,
                      """Ein Schriftschnitt, der durch einen Schriftstil charakterisiert
            wird."""@de ;
         rdfs:label "style Of"@en .


###  http://gams.uni-graz.at/o:typoo.ontology#subdivision
:subdivision rdf:type owl:ObjectProperty ;
             owl:inverseOf :subdivisionOf ;
             rdfs:comment """An Item Part that is a subdivision of an Item or a Function Area
            that is a subdivision of an Item Part."""@en ,
                          """Ein Exemplarteil, der eine Unterteilung eines Exemplars ist,
            oder ein Funktionsbereich, der eine Unterteilung eines Exemplarteils ist."""@de ;
             rdfs:label "Teilbereich"@de ,
                        "subdivision"@en .


###  http://gams.uni-graz.at/o:typoo.ontology#subdivisionOf
:subdivisionOf rdf:type owl:ObjectProperty ;
               rdfs:comment """An Item that is subdivided in Item Parts or an Item Part that is
            subdivided in Function Areas."""@en ,
                            """Ein Exemplar, das in Exemplarteile unterteilt ist, oder ein
            Exemplarteil, der in Funktionsbereiche unterteilt ist."""@de ;
               rdfs:label "Teilbereich von"@de ,
                          "subdivision Of"@en .


###  http://www.w3.org/2002/07/owl#topObjectProperty
owl:topObjectProperty rdf:type owl:ObjectProperty ,
                               owl:SymmetricProperty ,
                               owl:TransitiveProperty ,
                               owl:ReflexiveProperty .


#################################################################
#    Classes
#################################################################

###  http://gams.uni-graz.at/o:typoo.ontology#Allograph
:Allograph rdf:type owl:Class ;
           rdfs:subClassOf :CategoryScriptIndividuals ,
                           [ rdf:type owl:Restriction ;
                             owl:onProperty :manifestation ;
                             owl:allValuesFrom :Type
                           ] ,
                           [ rdf:type owl:Restriction ;
                             owl:onProperty :manifestationOf ;
                             owl:qualifiedCardinality "1"^^xsd:nonNegativeInteger ;
                             owl:onClass :Grapheme
                           ] ;
           rdfs:comment "A cultural or regional recognized form of graphically realizing a written unit , e.g. \"one-story a\" and \"two-story a\", \"Carolingian t\" and \"Roman t\""@en ,
                        "Eine von einer kulturhistorisch oder regional bedingten Schriftgemeinschaft anerkannte Form, eine schriftliche Einheit graphisch zu realisieren, z. B. \"einstöckiges a\" und \"zweistöckiges a\", \"karolingisches t\" und \"römisches t\""@de ;
           rdfs:label "Allograph"@de ,
                      "Allograph"@en .


###  http://gams.uni-graz.at/o:typoo.ontology#Apex
:Apex rdf:type owl:Class ;
      rdfs:subClassOf :TypeFragment ;
      rdfs:comment """Das Zusammentreffen von zwei Strichen (oft oben), z.B.
            \"A\", \"W\" und \"M\"."""@de ;
      rdfs:label "Apex"@en ,
                 "Scheitel"@de .


###  http://gams.uni-graz.at/o:typoo.ontology#Archigrapheme
:Archigrapheme rdf:type owl:Class ;
               rdfs:subClassOf :CategoryScriptIndividuals ,
                               [ rdf:type owl:Restriction ;
                                 owl:onProperty :manifestation ;
                                 owl:allValuesFrom :Grapheme
                               ] ;
               rdfs:comment "Einheit, zur Repräsentation der abstrakten Bedeutung eines Graphen, Allographen oder Graphems ohne Bindung an eine bestimmte Form"@de ,
                            "Unit that represents the abstract meaning of a graph, allograph or grapheme without being bound to a certain form"@en ;
               rdfs:label "Archigraphem"@de ,
                          "Archigrapheme"@en .


###  http://gams.uni-graz.at/o:typoo.ontology#Arm
:Arm rdf:type owl:Class ;
     rdfs:subClassOf :TypeFragment ;
     rdfs:comment "Querbalken (E, e, F, f, L)"@de ;
     rdfs:label "Arm"@de ,
                "Arm"@en .


###  http://gams.uni-graz.at/o:typoo.ontology#BodyText
:BodyText rdf:type owl:Class ;
          rdfs:subClassOf :FunctionArea ;
          rdfs:comment "Bereich/e des Mengentextes bzw. der Brotschrift."@de ;
          rdfs:label "Body Text"@en ,
                     "Mengenschrift"@de .


###  http://gams.uni-graz.at/o:typoo.ontology#Bow
:Bow rdf:type owl:Class ;
     rdfs:subClassOf :TypeFragment ;
     rdfs:comment """Form der Linien (z.B. \"gerundet\" oder
            \"flach\")."""@de ;
     rdfs:label "Bogen"@de ,
                "Bow"@en .


###  http://gams.uni-graz.at/o:typoo.ontology#BrokenLines
:BrokenLines rdf:type owl:Class ;
             rdfs:subClassOf :Lines ;
             owl:disjointWith :RoundedLines ;
             rdfs:comment "Broken lines (e.g. Blackletter typefaces)"@en ,
                          "Gebrochene Strichführung (z. B. Fraktur-Schriften)"@de ;
             rdfs:label "Broken Lines"@en ,
                        "Gebrochene Linienführung"@de .


###  http://gams.uni-graz.at/o:typoo.ontology#CategoryContext
:CategoryContext rdf:type owl:Class ;
                 owl:equivalentClass [ rdf:type owl:Class ;
                                       owl:unionOf ( :FunctionArea
                                                     :Item
                                                     :ItemPart
                                                   )
                                     ] ;
                 rdfs:comment "Context classes represent the textual and functional context in which a font occurs"@en ,
                              "Kontextklassen repräsentieren den textuellen und funktionellen Kontext, in dem ein Schriftschnitt verwendet wird"@de ;
                 rdfs:label "Category Context"@en ,
                            "Kategorie Kontext"@de .


###  http://gams.uni-graz.at/o:typoo.ontology#CategoryForm
:CategoryForm rdf:type owl:Class ;
              owl:equivalentClass [ rdf:type owl:Class ;
                                    owl:unionOf ( :ContrastModel
                                                  :FormPrinciple
                                                  :Lines
                                                  :Terminals
                                                )
                                  ] ;
              rdfs:comment "Form classes represent the conventional typographic design features of typefaces"@en ,
                           "Formklassen repräsentieren die konventionellen typografischen Gestaltungsmerkmale von Schriftarten"@de ;
              rdfs:label "Category Form"@en ,
                         "Kategorie Form"@de .


###  http://gams.uni-graz.at/o:typoo.ontology#CategoryScriptGroups
:CategoryScriptGroups rdf:type owl:Class ;
                      owl:equivalentClass [ rdf:type owl:Class ;
                                            owl:unionOf ( :Font
                                                          :Typeface
                                                        )
                                          ] ;
                      rdfs:comment "Schriftgruppenklassen repräsentieren Gruppierungen von singulären Schrifteinheiten"@de ,
                                   "Script Classes represent groupings of singular units of a typeface or font"@en ;
                      rdfs:label "Category Script Groups"@en ,
                                 "Kategorie Schriftgruppen"@de .


###  http://gams.uni-graz.at/o:typoo.ontology#CategoryScriptIndividuals
:CategoryScriptIndividuals rdf:type owl:Class ;
                           owl:equivalentClass [ rdf:type owl:Class ;
                                                 owl:unionOf ( :Allograph
                                                               :Archigrapheme
                                                               :FontType
                                                               :Grapheme
                                                               :Protograph
                                                               :Type
                                                             )
                                               ] ;
                           rdfs:comment "Schriftindividuenklassen repräsentieren Abstraktionsebenen singulärer Schrifteinheiten"@de ,
                                        "Script individual classes represent abstraction levels of single units of microtypography"@en ;
                           rdfs:label "Category Script Individuals"@en ,
                                      "Kategorie Schriftindividuen"@de .


###  http://gams.uni-graz.at/o:typoo.ontology#CategoryTypeMorphology
:CategoryTypeMorphology rdf:type owl:Class ;
                        owl:equivalentClass [ rdf:type owl:Class ;
                                              owl:unionOf ( :FragmentFeature
                                                            :TypeFragment
                                                          )
                                            ] ;
                        rdfs:comment "Typen Strukturklassen repräsentieren die morphologische Struktur einer Type und ihre Merkmale"@de ;
                        rdfs:label "Type Morphology"@en ,
                                   "Type structure classes represent the morphological structure of a type and its characteristics"@en ,
                                   "Typenmorphologie"@de .


###  http://gams.uni-graz.at/o:typoo.ontology#Cicero
:Cicero rdf:type owl:Class ;
        rdfs:subClassOf :Font ;
        rdfs:comment "Eine mittlere Schriftgrößen im Bleisatz. Sie hat eine Kegelhöhe von zwölf Didot-Punkten, das entspricht 4,512 mm"@de ;
        rdfs:label "Cicero"@de ,
                   "Cicero"@en .


###  http://gams.uni-graz.at/o:typoo.ontology#ContrastModel
:ContrastModel rdf:type owl:Class ;
               rdfs:subClassOf :CategoryForm ;
               rdfs:comment "Contrast model of strokes"@en ,
                            "Kontrastmodell der Striche"@de ;
               rdfs:label "Contrast Model"@en ,
                          "Kontrastmodell"@de .


###  http://gams.uni-graz.at/o:typoo.ontology#Counter
:Counter rdf:type owl:Class ;
         rdfs:subClassOf :TypeFragment ;
         rdfs:comment """Bereich, der ganz oder teilweise eingeschlossen ist, z.B.
            \"a\", \"p\" und \"c\"."""@de ;
         rdfs:label "Counter"@en ,
                    "Punze"@de .


###  http://gams.uni-graz.at/o:typoo.ontology#Crossbar
:Crossbar rdf:type owl:Class ;
          rdfs:subClassOf :TypeFragment ;
          rdfs:comment """Normalerweise ein horizontaler Strich (z.B. in \"A\" und
            \"H\")."""@de ;
          rdfs:label "Crossbar"@en ,
                     "Querbalken"@de .


###  http://gams.uni-graz.at/o:typoo.ontology#Decoration
:Decoration rdf:type owl:Class ;
            rdfs:subClassOf :FunctionArea ;
            rdfs:comment "Bereich der Zierschrift."@de ;
            rdfs:label "Decorative Type"@en ,
                       "Zierschrift"@de .


###  http://gams.uni-graz.at/o:typoo.ontology#DecorativeFormPrinciple
:DecorativeFormPrinciple rdf:type owl:Class ;
                         rdfs:subClassOf :FormPrinciple ;
                         rdfs:comment "Form principle of free or decorative fonts (e.g. Jugendstil fonts)"@en ,
                                      "Formprinzip freier bzw. dekorativer Schriften (z. B. Jugenstil-Schriften)"@de ;
                         rdfs:label "Decorative Form Principle"@en ,
                                    "Dekoratives Formprinzip"@de .


###  http://gams.uni-graz.at/o:typoo.ontology#Diagonal
:Diagonal rdf:type owl:Class ;
          rdfs:subClassOf :TypeFragment ;
          rdfs:comment """Diagonale Verbindung wie in \"N\", \"M\" oder
            \"Z\"."""@de ;
          rdfs:label "Diagonal"@en ,
                     "Diagonale"@de .


###  http://gams.uni-graz.at/o:typoo.ontology#DynamicFormPrinciple
:DynamicFormPrinciple rdf:type owl:Class ;
                      rdfs:subClassOf :FormPrinciple ;
                      rdfs:comment "Form principle of the broad nib with diagonal contrast axis with dynamic, open forms (Renaissance character with \"Garamond\" style)"@en ,
                                   "Formprinzip der Breitfeder mit schräg liegender Kontrastachse mit dynamischen, offenen Formen (Renaissance-Charakter im Stil der \"Garamond)\""@de ;
                      rdfs:label "Dynamic Form Principle"@en ,
                                 "Dynamisches Formprinzip"@de .


###  http://gams.uni-graz.at/o:typoo.ontology#Font
:Font rdf:type owl:Class ;
      rdfs:subClassOf :CategoryScriptGroups ,
                      [ rdf:type owl:Restriction ;
                        owl:onProperty :manifestationOf ;
                        owl:allValuesFrom :Typeface
                      ] ,
                      [ rdf:type owl:Restriction ;
                        owl:onProperty :part ;
                        owl:allValuesFrom :FontType
                      ] ;
      owl:disjointWith :Typeface ;
      rdfs:comment "A repertoire of printing types that have a uniform style (e.g. size and width), e.g. \"St-G font Cicero\", \"St-G font corpus\"."@en ,
                   "Ein Repertoire aus Drucktypen, das einen einheitlichen Schriftstil (z. B. Fette, Grad) hat, z. B. \"St-G-Schrift Cicero\", \"St-G-Schrift Korpus\""@de ;
      rdfs:label "Font"@en ,
                 "Schriftschnitt"@de .


###  http://gams.uni-graz.at/o:typoo.ontology#FontType
:FontType rdf:type owl:Class ;
          rdfs:subClassOf :CategoryScriptIndividuals ,
                          [ rdf:type owl:Restriction ;
                            owl:onProperty :partOf ;
                            owl:someValuesFrom :Font
                          ] ,
                          [ rdf:type owl:Restriction ;
                            owl:onProperty :manifestation ;
                            owl:qualifiedCardinality "1"^^xsd:nonNegativeInteger ;
                            owl:onClass :Protograph
                          ] ,
                          [ rdf:type owl:Restriction ;
                            owl:onProperty :manifestationOf ;
                            owl:qualifiedCardinality "1"^^xsd:nonNegativeInteger ;
                            owl:onClass :Type
                          ] ;
          rdfs:comment "A manifestation of a type in a certain typographic style, e.g. in a certain type size: \"t\" of the St-G font in Cicero; \"t\" of the St-G font in Petit."@en ,
                       "Eine Stilausprägung der Type in einem typografischen Stil, z.B. in einem bestimmten Schriftgrad: \"t\" der St-G-Schrift in Cicero; \"t\"der St-G-Schrift in Petit."@de ;
          rdfs:label "Drucktype"@de ,
                     "Font type"@en .


###  http://gams.uni-graz.at/o:typoo.ontology#FormPrinciple
:FormPrinciple rdf:type owl:Class ;
               rdfs:subClassOf :CategoryForm ;
               rdfs:comment "Form principle according to I. Kupferschmid (Buchstaben kommen selten allein: Ein typografisches Handbuch, 2. Aufl., Sulgen / Zürich 2004)"@en ,
                            "Formprinzip nach I. Kupferschmid (Buchstaben kommen selten allein: Ein typografisches Handbuch, 2. Aufl., Sulgen / Zürich 2004.)"@de ;
               rdfs:label "Form Principle"@en ,
                          "Formprinzip"@de .


###  http://gams.uni-graz.at/o:typoo.ontology#FragmentFeature
:FragmentFeature rdf:type owl:Class ;
                 rdfs:subClassOf :CategoryTypeMorphology ,
                                 [ rdf:type owl:Restriction ;
                                   owl:onProperty :featureOf ;
                                   owl:someValuesFrom :TypeFragment
                                 ] ;
                 owl:disjointWith :TypeFragment ;
                 rdfs:comment "Art der gestalterischen Modifikation des Fragments. Bsp.: „begradigt“, „spitz“, „verkürzt“"@de ,
                              "Type of design modification of the fragment. For example: \"straightened\", \"pointed\", \"shortened\""@en ;
                 rdfs:label "Feature"@en ,
                            "Merkmal"@de .


###  http://gams.uni-graz.at/o:typoo.ontology#FunctionArea
:FunctionArea rdf:type owl:Class ;
              rdfs:subClassOf :CategoryContext ;
              rdfs:comment "Der textuelle Funktionsbereich, in dem ein Protograph auftritt, z. B. \"Mengentext\", \"Titelseite\""@de ,
                           "The textual-functional context in which a protograph appears, e.g. \"body text\", \"title page\""@en ;
              rdfs:label "Function Area"@en ,
                         "Funktionsbereich"@de .


###  http://gams.uni-graz.at/o:typoo.ontology#GeometricFormPrinciple
:GeometricFormPrinciple rdf:type owl:Class ;
                        rdfs:subClassOf :FormPrinciple ;
                        rdfs:comment "Form principle of the redis nib without line contrast with constructed forms (geometric character in the style of \"Futura\")"@en ,
                                     "Formprinzip der Redisfeder ohne Strichkontrast mit konstruierten Formen (geometrischer Charakter im Stil der \"Futura\")"@de ;
                        rdfs:label "Geometric Form Principle"@en ,
                                   "Geometrisches Formprinzip"@de .


###  http://gams.uni-graz.at/o:typoo.ontology#Grapheme
:Grapheme rdf:type owl:Class ;
          rdfs:subClassOf :CategoryScriptIndividuals ,
                          [ rdf:type owl:Restriction ;
                            owl:onProperty :manifestation ;
                            owl:allValuesFrom :Allograph
                          ] ,
                          [ rdf:type owl:Restriction ;
                            owl:onProperty :manifestationOf ;
                            owl:qualifiedCardinality "1"^^xsd:nonNegativeInteger ;
                            owl:onClass :Archigrapheme
                          ] ;
          rdfs:comment "Differentiation between upper and lower case letters as the smallest distinctive linguistic unit of a written language system"@en ,
                       "Differenzierung zwischen Groß- und Kleinbuchstaben als kleinste bedeutungsunterscheidende Einheit eines Schriftsprachsystems. Bsp.: \"Minuskel g\" und \"Majuskel G\" in \"genossen\" und \"Genossen\""@de ;
          rdfs:label "Graphem"@de ,
                     "Grapheme"@en .


###  http://gams.uni-graz.at/o:typoo.ontology#Item
:Item rdf:type owl:Class ;
      rdfs:subClassOf :CategoryContext ,
                      [ rdf:type owl:Restriction ;
                        owl:onProperty :occurenceOf ;
                        owl:someValuesFrom :Font
                      ] ,
                      [ rdf:type owl:Restriction ;
                        owl:onProperty :occurenceOf ;
                        owl:someValuesFrom :FontType
                      ] ;
      rdfs:comment "Typografische Überlieferung, die man mittels bibliografischer und buchkundlicher Metadaten bestimmen kann"@de ,
                   "Typographical transmission, which can be determined by means of bibliographical and book-related metadata"@en ;
      rdfs:isDefinedBy "http://vocab.org/frbr/core#term-Item"^^xsd:anyURI ;
      rdfs:label "Exemplar"@de ,
                 "Item"@en .


###  http://gams.uni-graz.at/o:typoo.ontology#ItemPart
:ItemPart rdf:type owl:Class ;
          rdfs:subClassOf :CategoryContext ,
                          [ rdf:type owl:Restriction ;
                            owl:onProperty :subdivisionOf ;
                            owl:qualifiedCardinality "1"^^xsd:nonNegativeInteger ;
                            owl:onClass :Item
                          ] ;
          rdfs:comment "Sequence within a print, which can be indicated by a page interval and/or a description of the text part, e.g. \"Introduction, p. 3-5\""@en ,
                       "Sequenz innerhalb eines Drucks, die man durch ein Seitenintervall und/oder die Angabe einer Bezeichnung des Textteils angegeben kann, z. B. \"Einleitung, S. 3–5\""@de ;
          rdfs:label "Exemplarteil"@de ,
                     "Item Part"@en .


###  http://gams.uni-graz.at/o:typoo.ontology#ItemPartColophone
:ItemPartColophone rdf:type owl:Class ;
                   rdfs:subClassOf :ItemPart ;
                   rdfs:label "Kolophon"@de ,
                              "Kolophon"@en .


###  http://gams.uni-graz.at/o:typoo.ontology#ItemPartPoems
:ItemPartPoems rdf:type owl:Class ;
               rdfs:subClassOf :ItemPart ;
               rdfs:label "Gedichte"@de ,
                          "Poems"@en .


###  http://gams.uni-graz.at/o:typoo.ontology#ItemPartPreface
:ItemPartPreface rdf:type owl:Class ;
                 rdfs:subClassOf :ItemPart ;
                 rdfs:label "Preface"@en ,
                            "Vorwort"@de .


###  http://gams.uni-graz.at/o:typoo.ontology#ItemPartTitle
:ItemPartTitle rdf:type owl:Class ;
               rdfs:subClassOf :ItemPart ;
               rdfs:label "Titelblatt"@de ,
                          "Title Page"@en .


###  http://gams.uni-graz.at/o:typoo.ontology#Korpus
:Korpus rdf:type owl:Class ;
        rdfs:subClassOf :Font ;
        rdfs:comment "Eine mittlere Schriftgröße im Bleisatz. Sie hat eine Kegelhöhe von zehn Didot-Punkten, das entspricht 3,76 mm"@de ;
        rdfs:label "Corpus"@en ,
                   "Korpus"@de .


###  http://gams.uni-graz.at/o:typoo.ontology#LinearStroke
:LinearStroke rdf:type owl:Class ;
              rdfs:subClassOf :ContrastModel ;
              owl:disjointWith :StrokeContrast ;
              rdfs:comment "Linear strokes, i.e. no contrast (e.g. Grotesque typefaces)"@en ,
                           "Lineare Striche, d. h. kein Kontrast (z. B. Grotesk-Schriften)"@de ;
              rdfs:label "Linear Strokes"@en ,
                         "Lineare Striche"@de .


###  http://gams.uni-graz.at/o:typoo.ontology#Lines
:Lines rdf:type owl:Class ;
       rdfs:subClassOf :CategoryForm ;
       rdfs:comment "Linienführung der Striche"@de ,
                    "Style of lines"@en ;
       rdfs:label "Lines"@en ,
                  "Linienführung"@de .


###  http://gams.uni-graz.at/o:typoo.ontology#Petit
:Petit rdf:type owl:Class ;
       rdfs:subClassOf :Font ;
       rdfs:comment "Eine kleine Schriftgröße im Bleisatz. Sie hat eine Kegelhöhe von acht Didot-Punkten, das entspricht 3,008 mm"@de ;
       rdfs:label "Petit"@de ,
                  "Petit"@en .


###  http://gams.uni-graz.at/o:typoo.ontology#Protograph
:Protograph rdf:type owl:Class ;
            rdfs:subClassOf :CategoryScriptIndividuals ,
                            [ rdf:type owl:Restriction ;
                              owl:onProperty :manifestationOf ;
                              owl:someValuesFrom :FontType
                            ] ;
            rdfs:comment "Stellvertreter bzw. ‚Schablone‘ für alle im Druckerzeugnis gleichförmig erscheinenden Graphen, welche auf die gleiche Drucktype zurückgehen."@de ,
                         "Substitute or 'template' for all graphs appearing uniformly in the printed product, which are the result of various printing types."@en ;
            rdfs:label "Protograph"@de ,
                       "Protograph"@en .


###  http://gams.uni-graz.at/o:typoo.ontology#RoundedLines
:RoundedLines rdf:type owl:Class ;
              rdfs:subClassOf :Lines ;
              rdfs:comment "Abgerundete Linienführung (z. B. Antiqua-Schriften)"@de ,
                           "Rounded lines (e.g. Antiqua typefaces)"@en ;
              rdfs:label "Abgerundete Linienführung"@de ,
                         "Rounded Lines"@en .


###  http://gams.uni-graz.at/o:typoo.ontology#SansSerifs
:SansSerifs rdf:type owl:Class ;
            rdfs:subClassOf :Terminals ;
            owl:disjointWith :Serifs ;
            rdfs:comment "Serifenlose Endstrichbehandlung"@de ,
                         "Terminals without serifs"@en ;
            rdfs:label "Sans Serif"@en ,
                       "Serifenlos"@de .


###  http://gams.uni-graz.at/o:typoo.ontology#Serifs
:Serifs rdf:type owl:Class ;
        rdfs:subClassOf :Terminals ;
        rdfs:comment "Endstrichbehandlung mit Serifen"@de ,
                     "Terminals with serifs"@en ;
        rdfs:label "Serifen"@de ,
                   "Serifs"@en .


###  http://gams.uni-graz.at/o:typoo.ontology#Sides
:Sides rdf:type owl:Class ;
       rdfs:subClassOf :TypeFragment ;
       rdfs:comment """Gegenüberliegende senkrechte bzw. schräge Seiten, z.B. in
            \"W\", \"A\" und \"v\"."""@de ;
       rdfs:label "Schenkel"@de ,
                  "Sides"@en .


###  http://gams.uni-graz.at/o:typoo.ontology#StaticFormPrinciple
:StaticFormPrinciple rdf:type owl:Class ;
                     rdfs:subClassOf :FormPrinciple ;
                     rdfs:comment "Form principle of the pointed nib with vertical contrast axis and static, closed forms (classical character in the style of \"Bodoni\")"@en ,
                                  "Formprinzip der Spitzfeder mit senkrechter Kontrastachse und statischen, geschlossenen Formen (klassizistischer Charakter im Stil der \"Bodoni\")"@de ;
                     rdfs:label "Static Form Principle"@en ,
                                "Statisches Formprinzip"@de .


###  http://gams.uni-graz.at/o:typoo.ontology#Stem
:Stem rdf:type owl:Class ;
      rdfs:subClassOf :TypeFragment ;
      rdfs:comment "(Meist) senkrechte Linie."@de ;
      rdfs:label "Stamm"@de ,
                 "Stem"@en .


###  http://gams.uni-graz.at/o:typoo.ontology#StrokeContrast
:StrokeContrast rdf:type owl:Class ;
                rdfs:subClassOf :ContrastModel ;
                rdfs:comment "Lines with different widths (e.g. Antiqua typefaces)"@en ,
                             "Striche mit unterschiedlicher Breite (z. B. Antiqua-Schriften)"@de ;
                rdfs:label "Strichkontrast"@de ,
                           "Stroke Contrast"@en .


###  http://gams.uni-graz.at/o:typoo.ontology#Tail
:Tail rdf:type owl:Class ;
      rdfs:subClassOf :TypeFragment ;
      rdfs:comment """Abwärts gerichteter Strich, manchmal dekorativ, z.B. in
            \"Q\" oder \"G\"."""@de ;
      rdfs:label "Schweif"@de ,
                 "Tail"@en .


###  http://gams.uni-graz.at/o:typoo.ontology#Terminals
:Terminals rdf:type owl:Class ;
           rdfs:subClassOf :CategoryForm ;
           rdfs:comment "Design of terminals"@en ,
                        "Gestaltung der Endstriche"@de ;
           rdfs:label "Endstriche"@de ,
                      "Terminals"@en .


###  http://gams.uni-graz.at/o:typoo.ontology#Tertia
:Tertia rdf:type owl:Class ;
        rdfs:subClassOf :Font ;
        rdfs:comment "Eine mittlere Schriftgröße im Bleisatz. Sie hat eine Kegelhöhe von 16 Didot-Punkten, das entspricht 6,016 mm"@de ;
        rdfs:label "Tertia"@de ,
                   "Tertia"@en .


###  http://gams.uni-graz.at/o:typoo.ontology#Title
:Title rdf:type owl:Class ;
       rdfs:subClassOf :FunctionArea ;
       rdfs:comment "Bereich/e des ausgezeichneten Texts."@de ;
       rdfs:label "Titelschrift"@de ,
                  "Title Area"@en .


###  http://gams.uni-graz.at/o:typoo.ontology#Type
:Type rdf:type owl:Class ;
      rdfs:subClassOf :CategoryScriptIndividuals ,
                      [ rdf:type owl:Restriction ;
                        owl:onProperty :partOf ;
                        owl:someValuesFrom :Typeface
                      ] ,
                      [ rdf:type owl:Restriction ;
                        owl:onProperty :manifestation ;
                        owl:allValuesFrom :FontType
                      ] ,
                      [ rdf:type owl:Restriction ;
                        owl:onProperty :structure ;
                        owl:allValuesFrom :TypeFragment
                      ] ,
                      [ rdf:type owl:Restriction ;
                        owl:onProperty :manifestationOf ;
                        owl:qualifiedCardinality "1"^^xsd:nonNegativeInteger ;
                        owl:onClass :Allograph
                      ] ;
      rdfs:comment "A typographically individual allographical form within a typeface. Slight structural modifications of the allograph form can also be part of the type design, e.g: \"A\" the Garamond, \"A\" the Akzidenz-Grotesk, \"A\" the St-G typeface (with flat vertex)"@en ,
                   "Eine mit typografischen Mitteln gestaltete Allographenform. Auch leichte strukturelle Modifikationen der Allographenform können zur Gestaltung der Type zählen, z. B.: \"A\" der Garamond, \"A\" der Akzidenz-Grotesk, \"A\" der St-G-Schrift (mit flachem Scheitelpunkt)"@de ;
      rdfs:label "Type"@de ,
                 "Type"@en .


###  http://gams.uni-graz.at/o:typoo.ontology#TypeFragment
:TypeFragment rdf:type owl:Class ;
              rdfs:subClassOf :CategoryTypeMorphology ,
                              [ rdf:type owl:Restriction ;
                                owl:onProperty :feature ;
                                owl:someValuesFrom :FragmentFeature
                              ] ;
              rdfs:comment "Morphological component of the allograph form. For example: \"Tail\", \"Horizontal line\", \"Angle\", \"Arc\""@en ,
                           "Morphologischer Bestandteil der Allographenform. Bsp.: „Schweif“, „Querstrich“, „Winkel“, „Bogen“"@de ;
              rdfs:label "Fragment"@de ,
                         "Fragment"@en .


###  http://gams.uni-graz.at/o:typoo.ontology#Typeface
:Typeface rdf:type owl:Class ;
          rdfs:subClassOf :CategoryScriptGroups ,
                          [ rdf:type owl:Restriction ;
                            owl:onProperty :manifestation ;
                            owl:allValuesFrom :Font
                          ] ,
                          [ rdf:type owl:Restriction ;
                            owl:onProperty :part ;
                            owl:allValuesFrom :Type
                          ] ,
                          [ rdf:type owl:Restriction ;
                            owl:onProperty :formFeature ;
                            owl:qualifiedCardinality "1"^^xsd:nonNegativeInteger ;
                            owl:onClass :ContrastModel
                          ] ,
                          [ rdf:type owl:Restriction ;
                            owl:onProperty :formFeature ;
                            owl:qualifiedCardinality "1"^^xsd:nonNegativeInteger ;
                            owl:onClass :FormPrinciple
                          ] ,
                          [ rdf:type owl:Restriction ;
                            owl:onProperty :formFeature ;
                            owl:qualifiedCardinality "1"^^xsd:nonNegativeInteger ;
                            owl:onClass :Lines
                          ] ,
                          [ rdf:type owl:Restriction ;
                            owl:onProperty :formFeature ;
                            owl:qualifiedCardinality "1"^^xsd:nonNegativeInteger ;
                            owl:onClass :Terminals
                          ] ;
          rdfs:comment "A intentionally composed repertoire of types designed according to a uniform typographic pattern (e.g. shape of serifs, stroke contrast), e.g. \"St-G typeface\", \"Garamond\""@en ,
                       "Ein bewusst zusammengesetztes Repertoire aus Typen, die nach einem einheitlichen typografischen Formenschema (z. B. Form der Serifen, Strichkontrast) gestaltet sind, z. B. \"St-G-Schrift\", \"Garamond\""@de ;
          rdfs:label "Schriftart"@de ,
                     "Typeface"@en .


###  http://gams.uni-graz.at/o:typoo.ontology#VariousSizes
:VariousSizes rdf:type owl:Class ;
              rdfs:subClassOf :Font ;
              rdfs:comment "Verschiedene Größen, oft in dekorativen Zierschriften"@de ;
              rdfs:label "Various Sizes"@en ,
                         "Verschiedene Schriftgrößen"@de .


#################################################################
#    Annotations
#################################################################

:Satztrenner rdfs:label "Satztrenner" .


owl:Thing rdfs:label "Mikrotypografie"@de ,
                     "Microtypography"@en .


#################################################################
#    General axioms
#################################################################

[ rdf:type owl:AllDisjointClasses ;
  owl:members ( :Allograph
                :Archigrapheme
                :FontType
                :Grapheme
                :Protograph
                :Type
              )
] .


[ rdf:type owl:AllDisjointClasses ;
  owl:members ( :Apex
                :Arm
                :Bow
                :Counter
                :Crossbar
                :Diagonal
                :Sides
                :Stem
                :Tail
              )
] .


[ rdf:type owl:AllDisjointClasses ;
  owl:members ( :BodyText
                :Decoration
                :Title
              )
] .


[ rdf:type owl:AllDisjointClasses ;
  owl:members ( :Cicero
                :Korpus
                :Petit
                :Tertia
              )
] .


[ rdf:type owl:AllDisjointClasses ;
  owl:members ( :Cicero
                :Korpus
                :Tertia
              )
] .


[ rdf:type owl:AllDisjointClasses ;
  owl:members ( :ContrastModel
                :FormPrinciple
                :Lines
                :Terminals
              )
] .


[ rdf:type owl:AllDisjointClasses ;
  owl:members ( :DecorativeFormPrinciple
                :DynamicFormPrinciple
                :GeometricFormPrinciple
                :StaticFormPrinciple
              )
] .


[ rdf:type owl:AllDisjointClasses ;
  owl:members ( :FunctionArea
                :Item
                :ItemPart
              )
] .


[ rdf:type owl:AllDisjointClasses ;
  owl:members ( :ItemPartColophone
                :ItemPartPoems
                :ItemPartPreface
                :ItemPartTitle
              )
] .


###  Generated by the OWL API (version 4.2.8.20170104-2310) https://github.com/owlcs/owlapi
